Intermediate commit

src/ReactorModel/Execution/Basic.lean
@@ -23,41 +23,67 @@ inductive Apply.RTC : Reaction.Output → State α → State α → Type
 notation s₁:max " -[" cs "]→ " s₂:max => Apply.RTC cs s₁ s₂
 
 inductive Skip : State α → State α → Type
-  | mk : (Allows s rcn) → (¬Triggers s rcn) → (s.clock ≤ t) → Skip s (s.at t |>.record rcn)
+  | mk : (Allows s rcn) → (¬Triggers s rcn) → (s.clock ≤ t) → Skip s (s.record rcn |>.at t)
 
-notation s₁:max " ↓ₛ " s₂:max => Skip s₁ s₂
+notation s₁:max " ↓ˢ " s₂:max => Skip s₁ s₂
 
 inductive Exec : State α → State α → Type
   | mk : (Allows s₁ rcn) → (Triggers s₁ rcn) → (s₁ -[s₁.output rcn]→ s₂) → (s₁.clock ≤ t) → 
-         Exec s₁ (s₂.at t |>.record rcn)
+         Exec s₁ (s₂.record rcn |>.at t)
 
-notation s₁:max " ↓ₑ " s₂:max => Exec s₁ s₂
+notation s₁:max " ↓ᵉ " s₂:max => Exec s₁ s₂
 
-inductive Time : State α → State α → Type
+inductive Tag : State α → State α → Type
   | mk : (Closed s) → (NextTag s g) → (Refresh s.rtr ref $ s.logicals g) → (g.time ≤ t) → 
-         Time s { s with rtr := ref, tag := g, clock := t, progress := ∅ }
+         (s.clock ≤ t) → Tag s { s with rtr := ref, tag := g, clock := t, progress := ∅ }
 
-notation s₁:max " ↓ₜ " s₂:max => Time s₁ s₂
+notation s₁:max " ↓ᵗ " s₂:max => Tag s₁ s₂
 
-inductive Phys : State α → State α → Type
-  | mk {phy : ID} : Phys s s -- TODO
+inductive Clock : State α → State α → Type
+  | mk : (s.clock < t) → Clock s (s.at t)  
 
-notation s₁:max " ↓ₚ " s₂:max => Exec s₁ s₂
+notation s₁:max " ↓ᶜ " s₂:max => Clock s₁ s₂
+
+-- TODO: Rename this to `Tick`?
+inductive Sync (s₁ s₂ : State α)
+  | skip  (s : s₁ ↓ˢ s₂)
+  | exec  (e : s₁ ↓ᵉ s₂)
+  | tag   (t : s₁ ↓ᵗ s₂)
+  | clock (c : s₁ ↓ᶜ s₂)
 
 end Step
 
-inductive Step (s₁ s₂ : State α) : Prop
-  | skip (s : s₁ ↓ₛ s₂)
-  | exec (e : s₁ ↓ₑ s₂)
-  | time (t : s₁ ↓ₜ s₂)
-  | phys (p : s₁ ↓ₚ s₂)
+-- TODO: I'm inclined to remove the notion of a `clock` step and intepret each of the remaining sync
+--       steps as meaning "somewhere in the physical time span s₁.clock to s₂.clock the step was
+--       performed". The only problem with removing the `clock` step is that we can only schedule
+--       physical actions in parallel to *some* sync step existing. Is this a problem? I think the 
+--       answer might be related to how termination of reactors works in a setting where we have
+--       physical time. Cause wouldnt such a reactor never terminate, as there might still be a
+--       physical action scheduled at some point in the future.
+--       Side Note: If you remove `clock` step, rename the `Sync` steps back to `Logical` and 
+--                  have the indices be subscripts.
+
+inductive Step : State α → State α → Type
+  | sync : (Step.Sync s₁ s₂) → Step s₁ s₂
+  | phys : (Step.Sync s₁ s₂) → (i ∈ s₁.rtr[.phy]) → (s₁.clock ≤ t) → (t ≤ s₂.clock) → 
+            Step s₁ (s₂.schedule .phy i t v)
 
 notation s₁:max " ↓ " s₂:max => Step s₁ s₂
 
 end Execution
 
-inductive Execution : State α → State α → Prop
+inductive Execution : State α → State α → Type
   | refl  : Execution s s
   | trans : (s₁ ↓ s₂) → (Execution s₂ s₃) → Execution s₁ s₃
 
-notation s₁ " ⇓ " s₂ => Execution s₁ s₂
+notation s₁ " ↓* " s₂ => Execution s₁ s₂
+
+-- TODO: Would it be nice/useful to have a notion of events?
+--       Perhaps `Change`s are something like "instantaneous events"?
+
+-- TODO: Move this to Theorems/Execution.lean once that file builds again.
+-- TODO: If a list is impractical to work with, you could also return a map Time ⇀ (ID × Value).
+noncomputable def Execution.physicalEvents {s₁ : State α} : (s₁ ↓* s₂) → List (Time × ID × Value) 
+  | refl => []
+  | trans (.sync _) tl => tl.physicalEvents
+  | trans (.phys (t := t) (i := i) (v := v) ..) tl => (t, i, v) :: tl.physicalEvents
