src/ReactorModel/Execution/Theorems/Step/Exec.lean
@@ -6,43 +6,49 @@ namespace Execution.Step.Exec
 
 variable [Hierarchical α] {s₁ : State α}
 
-def rcn :                  (s₁ ↓ₑ s₂) → ID                               | mk (rcn := r) .. => r
-def applied :              (s₁ ↓ₑ s₂) → State α                          | mk (s₂ := s) .. => s
-theorem allows_rcn :   (e : s₁ ↓ₑ s₂) → Allows s₁ e.rcn                  | mk a .. => a
-theorem triggers_rcn : (e : s₁ ↓ₑ s₂) → Triggers s₁ e.rcn                | mk _ t _ => t
-theorem apply :        (e : s₁ ↓ₑ s₂) → s₁ -[s₁.output e.rcn]→ e.applied | mk _ _ a => a
-theorem dst_eq :       (e : s₁ ↓ₑ s₂) → s₂ = e.applied.record e.rcn      | mk .. => rfl
+def rcn :                  (s₁ ↓ᵉ s₂) → ID                                       | mk (rcn := r) .. => r
+def clock :                (s₁ ↓ᵉ s₂) → _root_.Time                              | mk (t := t) .. => t
+def applied :              (s₁ ↓ᵉ s₂) → State α                                  | mk (s₂ := s) .. => s
+theorem allows_rcn :   (e : s₁ ↓ᵉ s₂) → Allows s₁ e.rcn                          | mk a .. => a
+theorem triggers_rcn : (e : s₁ ↓ᵉ s₂) → Triggers s₁ e.rcn                        | mk _ t .. => t
+theorem apply :        (e : s₁ ↓ᵉ s₂) → s₁ -[s₁.output e.rcn]→ e.applied         | mk _ _ a _ => a
+theorem clock_le :     (e : s₁ ↓ᵉ s₂) → s₁.clock ≤ e.clock                       | mk _ _ _ c => c
+theorem dst_eq :       (e : s₁ ↓ᵉ s₂) → s₂ = (e.applied.at e.clock).record e.rcn | mk .. => rfl
 
-theorem applied_rtr_eq (e : s₁ ↓ₑ s₂) : e.applied.rtr = s₂.rtr := by
+theorem applied_rtr_eq (e : s₁ ↓ᵉ s₂) : e.applied.rtr = s₂.rtr := by
   cases e
-  simp [applied, record_preserves_rtr]
+  simp [applied, record_preserves_rtr, at_preserves_rtr]
 
-theorem preserves_tag (e : s₁ ↓ₑ s₂) : s₁.tag = s₂.tag := by
-  simp [e.dst_eq, State.record_preserves_tag, e.apply.preserves_tag]
+theorem preserves_tag (e : s₁ ↓ᵉ s₂) : s₁.tag = s₂.tag := by
+  simp [e.dst_eq, record_preserves_tag, e.apply.preserves_tag, at_preserves_tag]
 
-theorem equiv (e : s₁ ↓ₑ s₂) : s₁.rtr ≈ s₂.rtr := by
-  simp [e.dst_eq, State.record_preserves_rtr, e.apply.equiv]
+theorem equiv (e : s₁ ↓ᵉ s₂) : s₁.rtr ≈ s₂.rtr := by
+  simp [e.dst_eq, record_preserves_rtr, at_preserves_rtr, e.apply.equiv]
 
-theorem progress_eq (e : s₁ ↓ₑ s₂) : s₂.progress = s₁.progress.insert e.rcn := by 
-  simp [e.dst_eq, State.record_progress_eq, e.apply.preserves_progress]
+theorem progress_eq (e : s₁ ↓ᵉ s₂) : s₂.progress = s₁.progress.insert e.rcn := by 
+  simp [e.dst_eq, record_progress_eq, at_preserves_progress, e.apply.preserves_progress]
 
-theorem preserves_nontrivial {e : s₁ ↓ₑ s₂} (n : s₁.Nontrivial) : s₂.Nontrivial :=
+theorem preserves_nontrivial {e : s₁ ↓ᵉ s₂} (n : s₁.Nontrivial) : s₂.Nontrivial :=
   n.equiv e.equiv
 
-theorem indep_allows_iff (e : s₁ ↓ₑ s₂) (hi : i ≮[s₁.rtr]≯ e.rcn) : 
+theorem indep_allows_iff (e : s₁ ↓ᵉ s₂) (hi : i ≮[s₁.rtr]≯ e.rcn) : 
     s₁.Allows i ↔ s₂.Allows i := by
   have a := e.apply
-  simp [e.dst_eq, ←Allows.iff_record_indep (a.preserves_independent hi).symm, a.allows_iff]
+  replace hi := (at_preserves_rtr e.applied e.clock).symm ▸ a.preserves_independent hi
+  simp [
+    e.dst_eq, ←Allows.iff_record_indep hi.symm, ←Allows.iff_at (s := e.applied) (t := e.clock), 
+    a.allows_iff
+  ]
   
-theorem unprocessed_eq (e : s₁ ↓ₑ s₂) : s₂.unprocessed = s₁.unprocessed \ {e.rcn} := by
+theorem unprocessed_eq (e : s₁ ↓ᵉ s₂) : s₂.unprocessed = s₁.unprocessed \ {e.rcn} := by
   ext i
   simp [State.unprocessed, Equivalent.obj?_rcn_eq e.equiv, and_assoc, e.progress_eq]
   intro _; simp [Set.insert]; push_neg; simp [and_comm]
 
-theorem rcn_mem_unprocessed (e : s₁ ↓ₑ s₂) : e.rcn ∈ s₁.unprocessed := 
+theorem rcn_mem_unprocessed (e : s₁ ↓ᵉ s₂) : e.rcn ∈ s₁.unprocessed := 
   ⟨e.allows_rcn.mem, e.allows_rcn.unprocessed⟩ 
 
-theorem unprocessed_ssubset (e : s₁ ↓ₑ s₂) : s₂.unprocessed ⊂ s₁.unprocessed := by
+theorem unprocessed_ssubset (e : s₁ ↓ᵉ s₂) : s₂.unprocessed ⊂ s₁.unprocessed := by
   simp [e.unprocessed_eq, Set.ssubset_iff_subset_ne]
   exact e.rcn_mem_unprocessed
 
@@ -53,7 +59,7 @@ namespace Execution.Step.Exec
 variable [Proper α] {s s₁ : State α} {rcn : Reaction}
 
 theorem indep_restriction_eq  
-    (e : s₁ ↓ₑ s₂) (hi : e.rcn ≮[s₁.rtr]≯ i) (ho : s₁.rtr[.rcn][i] = some rcn) : 
+    (e : s₁ ↓ᵉ s₂) (hi : e.rcn ≮[s₁.rtr]≯ i) (ho : s₁.rtr[.rcn][i] = some rcn) : 
     input.restriction s₁ rcn cpt = input.restriction s₂ rcn cpt := by 
   simp [input.restriction]
   apply Partial.ext_restrict 
@@ -61,36 +67,37 @@ theorem indep_restriction_eq
   exact e.applied_rtr_eq ▸ e.apply.preserves_unchanged $ State.target_not_mem_indep_output ho hi hd
 
 theorem indep_input_eq 
-    (e : s₁ ↓ₑ s₂) (hi : e.rcn ≮[s₁.rtr]≯ i) (h₁ : s₁.rtr[.rcn][i] = some rcn)
+    (e : s₁ ↓ᵉ s₂) (hi : e.rcn ≮[s₁.rtr]≯ i) (h₁ : s₁.rtr[.rcn][i] = some rcn)
     (h₂ : s₂.rtr[.rcn][i] = some rcn) : s₁.input i = s₂.input i := by 
   simp [input, h₁, h₂]
   refine ⟨?_, e.preserves_tag⟩
   ext1
   exact e.indep_restriction_eq hi h₁
 
-theorem indep_output_eq (e : s₁ ↓ₑ s₂) (hi : e.rcn ≮[s₁.rtr]≯ i) : s₁.output i = s₂.output i := by 
+theorem indep_output_eq (e : s₁ ↓ᵉ s₂) (hi : e.rcn ≮[s₁.rtr]≯ i) : s₁.output i = s₂.output i := by 
   simp [output]
   have he := Equivalent.obj?_rcn_eq e.equiv
   cases h : s₁.rtr[.rcn][i] <;> simp [he ▸ h]
   simp [e.indep_input_eq hi h $ he ▸ h]
 
 theorem indep_comm 
-    (e₁ : s ↓ₑ s₁) (e₁₂ : s₁ ↓ₑ s₁₂) (e₂ : s ↓ₑ s₂) (e₂₁ : s₂ ↓ₑ s₂₁) 
+    (e₁ : s ↓ᵉ s₁) (e₁₂ : s₁ ↓ᵉ s₁₂) (e₂ : s ↓ᵉ s₂) (e₂₁ : s₂ ↓ᵉ s₂₁) 
     (hr₁ : e₁.rcn = e₂₁.rcn) (hr₂ : e₂.rcn = e₁₂.rcn) (hi : e₁.rcn ≮[s.rtr]≯ e₂.rcn) : 
-    s₁₂ = s₂₁ := by 
+    s₁₂ ≈ s₂₁ := by 
   have ho₁ := e₁.indep_output_eq hi
   have ho₂ := e₂.indep_output_eq hi.symm
   cases e₁; cases e₁₂; cases e₂; cases e₂₁
-  case _ rcn₁ s₁ _ _ a₁ rcn₂ s₁₂ _ _ a₁₂ _ s₂ _ _ a₂ _ s₂₁ _ _ a₂₁ => 
+  case _ rcn₁ s₁ t₁ _ _ a₁ ht₁ rcn₂ s₁₂ t₁₂ _ _ a₁₂ ht₁₂ _ s₂ t₂ _ _ a₂ ht₂ _ s₂₁ t₂₁ _ _ a₂₁ ht₂₁ => 
     cases hr₁; cases hr₂; simp [Exec.rcn] at *
     have ⟨z₁₂, f₁₂⟩ := Apply.RTC.construct s₁ (s.output rcn₂)
     have ⟨z₂₁, f₂₁⟩ := Apply.RTC.construct s₂ (s.output rcn₁)
     rw [←ho₁] at a₁₂; rw [←ho₂] at a₂₁
-    cases f₁₂.comm_record a₁₂; cases f₂₁.comm_record a₂₁
-    rw [record_comm]; congr
-    exact Apply.RTC.disjoint_targets_comm (s.indep_output_disjoint_targets hi) a₁ f₁₂ a₂ f₂₁
+    sorry 
+    -- cases f₁₂.comm_record a₁₂; cases f₂₁.comm_record a₂₁
+    -- rw [record_comm]; congr
+    -- exact Apply.RTC.disjoint_targets_comm (s.indep_output_disjoint_targets hi) a₁ f₁₂ a₂ f₂₁
 
-theorem indep_triggers_iff (e : s₁ ↓ₑ s₂) (hi : i ≮[s₁.rtr]≯ e.rcn) : 
+theorem indep_triggers_iff (e : s₁ ↓ᵉ s₂) (hi : i ≮[s₁.rtr]≯ e.rcn) : 
     s₁.Triggers i ↔ s₂.Triggers i := by
   constructor <;> intro ⟨ho, ht⟩  
   case mp =>
