src/ReactorModel/Execution/Theorems/Step/Skip.lean
@@ -7,42 +7,48 @@ namespace Execution.Step.Skip
 
 variable [Hierarchical α] {s₁ : State α}
 
-def rcn :                      (s₁ ↓ₛ s₂) → ID                   | mk (rcn := rcn) .. => rcn
-theorem allows_rcn :       (e : s₁ ↓ₛ s₂) → Allows s₁ e.rcn      | mk a _ => a
-theorem not_triggers_rcn : (e : s₁ ↓ₛ s₂) → ¬Triggers s₁ e.rcn   | mk _ t => t
-theorem dst_eq :           (e : s₁ ↓ₛ s₂) → s₂ = s₁.record e.rcn | mk .. => rfl
+def rcn :                      (s₁ ↓ˢ s₂) → ID                                | mk (rcn := rcn) .. => rcn
+def clock :                    (s₁ ↓ˢ s₂) → _root_.Time                       | mk (t := t) .. => t
+theorem allows_rcn :       (e : s₁ ↓ˢ s₂) → Allows s₁ e.rcn                   | mk a .. => a
+theorem not_triggers_rcn : (e : s₁ ↓ˢ s₂) → ¬Triggers s₁ e.rcn                | mk _ t _ => t
+theorem clock_le :         (e : s₁ ↓ˢ s₂) → s₁.clock ≤ e.clock                | mk _ _ c => c
+theorem dst_eq :           (e : s₁ ↓ˢ s₂) → s₂ = (s₁.at e.clock).record e.rcn | mk .. => rfl
 
-theorem preserves_rtr (e : s₁ ↓ₛ s₂) : s₁.rtr = s₂.rtr := by
-  simp [e.dst_eq, State.record_preserves_rtr]
+theorem preserves_rtr (e : s₁ ↓ˢ s₂) : s₁.rtr = s₂.rtr := by
+  simp [e.dst_eq, record_preserves_rtr, at_preserves_rtr]
 
-theorem preserves_tag (e : s₁ ↓ₛ s₂) : s₁.tag = s₂.tag := by
-  simp [e.dst_eq, State.record_preserves_tag]
+theorem preserves_tag (e : s₁ ↓ˢ s₂) : s₁.tag = s₂.tag := by
+  simp [e.dst_eq, record_preserves_tag, at_preserves_tag]
 
-theorem preserves_events (e : s₁ ↓ₛ s₂) : s₁.events = s₂.events := by
-  simp [e.dst_eq, State.record_preserves_events]
+theorem preserves_events (e : s₁ ↓ˢ s₂) : s₁.events = s₂.events := by
+  simp [e.dst_eq, record_preserves_events, at_preserves_events]
 
-theorem equiv (e : s₁ ↓ₛ s₂) : s₁.rtr ≈ s₂.rtr := by
-  simp [e.dst_eq, State.record_preserves_rtr]
+theorem equiv (e : s₁ ↓ˢ s₂) : s₁.rtr ≈ s₂.rtr := by
+  simp [e.dst_eq, record_preserves_rtr, at_preserves_rtr]
   exact .refl _
 
-theorem progress_eq (e : s₁ ↓ₛ s₂) : s₂.progress = s₁.progress.insert e.rcn := by 
-  simp [e.dst_eq, State.record_progress_eq]
+theorem progress_eq (e : s₁ ↓ˢ s₂) : s₂.progress = s₁.progress.insert e.rcn := by 
+  simp [e.dst_eq, at_preserves_progress, record_progress_eq]
 
-theorem preserves_nontrivial {e : s₁ ↓ₛ s₂} (n : s₁.Nontrivial) : s₂.Nontrivial :=
+theorem preserves_nontrivial {e : s₁ ↓ˢ s₂} (n : s₁.Nontrivial) : s₂.Nontrivial :=
   n.equiv e.equiv
 
-theorem indep_allows_iff (e : s₁ ↓ₛ s₂) (hi : i ≮[s₁.rtr]≯ e.rcn) : 
+theorem indep_allows_iff (e : s₁ ↓ˢ s₂) (hi : i ≮[s₁.rtr]≯ e.rcn) : 
     s₁.Allows i ↔ s₂.Allows i := by
-  simp [e.dst_eq, Allows.iff_record_indep hi.symm]
+  simp [e.dst_eq, Allows.iff_record_indep hi.symm, Allows.iff_at (s := s₁.record _) (t := e.clock)]
+  rfl
 
-theorem triggers_iff (e : s₁ ↓ₛ s₂) : 
-    s₁.Triggers i ↔ s₂.Triggers i := by
-  simp [e.dst_eq, Triggers.iff_record (s := s₁) (i₁ := e.rcn)]
+theorem triggers_iff (e : s₁ ↓ˢ s₂) : s₁.Triggers i ↔ s₂.Triggers i := by
+  simp [
+    e.dst_eq, Triggers.iff_record (s := s₁) (i₁ := e.rcn), 
+    Triggers.iff_at (s := s₁.record _) (t := e.clock)
+  ]
+  rfl
 
 theorem comm 
-    (e₁ : s ↓ₛ s₁) (e₁₂ : s₁ ↓ₛ s₁₂) (e₂ : s ↓ₛ s₂) (e₂₁ : s₂ ↓ₛ s₂₁) (hr₁ : e₁.rcn = e₂₁.rcn) 
-    (hr₂ : e₂.rcn = e₁₂.rcn) : s₁₂ = s₂₁ := by 
-  ext1
+    (e₁ : s ↓ˢ s₁) (e₁₂ : s₁ ↓ˢ s₁₂) (e₂ : s ↓ˢ s₂) (e₂₁ : s₂ ↓ˢ s₂₁) (hr₁ : e₁.rcn = e₂₁.rcn) 
+    (hr₂ : e₂.rcn = e₁₂.rcn) : s₁₂ ≈ s₂₁ := by 
+  constructor
   case rtr => 
     exact e₁₂.preserves_rtr ▸ e₁.preserves_rtr ▸ e₂₁.preserves_rtr ▸ e₂.preserves_rtr 
   case tag => 
@@ -56,15 +62,15 @@ theorem comm
     simp [h₁, h₂]
     apply Set.insert_comm
 
-theorem unprocessed_eq (e : s₁ ↓ₛ s₂) : s₂.unprocessed = s₁.unprocessed \ {e.rcn} := by
+theorem unprocessed_eq (e : s₁ ↓ˢ s₂) : s₂.unprocessed = s₁.unprocessed \ {e.rcn} := by
   ext i
   simp [State.unprocessed, Equivalent.obj?_rcn_eq e.equiv, and_assoc, e.progress_eq]
   intro _; simp [Set.insert]; push_neg; simp [and_comm]
 
-theorem rcn_mem_unprocessed (e : s₁ ↓ₛ s₂) : e.rcn ∈ s₁.unprocessed := 
+theorem rcn_mem_unprocessed (e : s₁ ↓ˢ s₂) : e.rcn ∈ s₁.unprocessed := 
   ⟨e.allows_rcn.mem, e.allows_rcn.unprocessed⟩ 
 
-theorem unprocessed_ssubset (e : s₁ ↓ₛ s₂) : s₂.unprocessed ⊂ s₁.unprocessed := by
+theorem unprocessed_ssubset (e : s₁ ↓ˢ s₂) : s₂.unprocessed ⊂ s₁.unprocessed := by
   simp [e.unprocessed_eq, Set.ssubset_iff_subset_ne]
   exact e.rcn_mem_unprocessed
 
