src/ReactorModel/Execution/Theorems/Execution.lean
@@ -5,10 +5,11 @@ open Classical Reactor
 
 namespace Execution
 
-variable [Proper α] {s : State α}
+variable [Proper α] {s s₁ s₂ : State α}
 
 theorem deterministic 
-    (e₁ : s ⇓ s₁) (e₂ : s ⇓ s₂) (ht : s₁.tag = s₂.tag) (hp : s₁.progress = s₂.progress) : s₁ = s₂ := 
+    (e₁ : s ↓* s₁) (e₂ : s ↓* s₂) (ht : s₁.tag = s₂.tag) (hp : s₁.progress = s₂.progress) 
+    (he : e₁.physicalEvents = e₂.physicalEvents) : s₁ = s₂ := 
   if h : s.Nontrivial 
   then (e₁.to_grouped h).some.deterministic h ht hp (e₂.to_grouped h).some
   else e₁.trivial_deterministic h e₂ ht
